blend recursive definition seamlessly into glorious state machine

immutable-btree/BtreeSpec.dfy
@@ -18,12 +18,6 @@ abstract module BtreeSpec {
   predicate Init(k: Constants, s: Variables) {
   }
 
-  datatype Step =
-    | GetStep(key: Key, value: Value, lookup: Lookup)
-    | PutStep(key: Key, value: Value, lookup: Lookup)
-    | SplitStep()
-    | GrowStep()
-
   datatype Layer<Value(!new)> = Layer(lb: Key, ub: Key, node: Node<Value>, slot: int)
   type Lookup<Value(!new)> = seq<Layer<Value>>
 
@@ -33,17 +27,46 @@ abstract module BtreeSpec {
     && s' == s
   }
 
-  predicate Put(k: Constants, s: Variables, s': Variables, key: Key, value: Value, lookup: Lookup)
+  predicate PutTransform(tree:Node, newtree:Node, key:Key, value:Value)
+    decreases tree;
   {
-    
+    if tree.Leaf? then (
+      var pos := Keyspace.LargestLte(tree.keys, query);
+      if pos >= 0 && query == tree.keys[pos] (
+        newtree == Leaf(tree.keys, tree.values[pos := value]);
+      ) else (
+        var newkeys := tree.keys[..pos+1] + [query] + tree.keys[pos+1..];
+        var newvals := tree.values[..pos+1] + [value] + tree.values[pos+1..];
+        newtree == Leaf(newkeys, newvals);
+      )
+    ) else (
+      var pos := Keyspace.LargestLte(tree.pivots, query) + 1;
+      var newlb := LeftBound(lb, tree.pivots, tree.children, pos);
+      var newub := RightBound(tree.pivots, tree.children, ub, pos);
+
+      // Before we can call Define recursively, we must prove that the child CantEquivocate.
+      var newchild := PutTransform(newlb, tree.children[pos], newub, query, value);
+      newtree := Index(tree.pivots, tree.children[pos := newchild]);
+    )
   }
+
+  predicate Put(k: Constants, s: Variables, s': Variables, key: Key, value: Value)
+  {
+    && PutTransform(s.root, s'.root, key, value)
+  }
+
+  datatype Step =
+    | GetStep(key: Key, value: Value, lookup: Lookup)
+    | PutStep(key: Key, value: Value)
+    | SplitStep()
+    | GrowStep()
 
   predicate NextStep(k: Constants, s: Variables, s': Variables, step:Step) {
     match step {
       case GetStep(key, value, lookup) => Get(k, s, s', key, value, lookup)
-      case PutStep() => 
-      case SplitStep() => 
-      case GrowStep() => 
+      case PutStep() => Put(k, s, s', key, value)
+      case SplitStep() => Split(k, s, s')
+      case GrowStep() => GrowStep(k, s, s')
     }
   }
 
